Move things to ExprInversion

src/Reflection/Syntax.v
@@ -375,35 +375,6 @@ Section language.
            end.
     End map.
 
-    Section misc.
-      Definition invert_Const {var t} (e : @exprf var t) : option (interp_type t)
-        := match e with Const _ v => Some v | _ => None end.
-      Definition invert_Var {var t} (e : @exprf var (Tbase t)) : option (var t)
-        := match e in @exprf _ t' return option (var match t' with
-                                                     | Tbase t' => t'
-                                                     | _ => t
-                                                     end)
-           with
-           | Var _ v => Some v
-           | _ => None
-           end.
-      Definition invert_Op {var t} (e : @exprf var t) : option { t1 : flat_type & op t1 t * exprf t1 }%type
-        := match e with Op _ _ opc args => Some (existT _ _ (opc, args)) | _ => None end.
-      Definition invert_LetIn {var A} (e : @exprf var A) : option { B : _ & exprf B * (interp_flat_type_gen var B -> exprf A) }%type
-        := match e in @exprf _ t return option { B : _ & _ * (_ -> exprf t) }%type with
-           | LetIn _ ex _ eC => Some (existT _ _ (ex, eC))
-           | _ => None
-           end.
-      Definition invert_Pair {var A B} (e : @exprf var (Prod A B)) : option (exprf A * exprf B)
-        := match e in @exprf _ t return option match t with
-                                               | Prod _ _ => _
-                                               | _ => unit
-                                               end with
-           | Pair _ x _ y => Some (x, y)%core
-           | _ => None
-           end.
-    End misc.
-
     Section wf.
       Context {var1 var2 : base_type_code -> Type}.
 
@@ -508,11 +479,6 @@ Global Arguments Wf {_ _ _ t} _.
 Global Arguments Interp {_ _ _} interp_op {t} _.
 Global Arguments interp {_ _ _} interp_op {t} _.
 Global Arguments interpf {_ _ _} interp_op {t} _.
-Global Arguments invert_Const {_ _ _ _ _} _.
-Global Arguments invert_Var {_ _ _ _ _} _.
-Global Arguments invert_Op {_ _ _ _ _} _.
-Global Arguments invert_LetIn {_ _ _ _ _} _.
-Global Arguments invert_Pair {_ _ _ _ _ _} _.
 
 Module Export Notations.
   Notation "A * B" := (@Prod _ A B) : ctype_scope.
